cava/arrow-examples/Mux2_1.v
@@ -42,9 +42,9 @@ Definition mux2_1 Cava := toCava Cava (Closure_conversion mux2_1').
 Local Open Scope string_scope.
 
 Definition mux2_1_Interface :=
-   mkCombinationalInterface "mux2_1"
-     (Tuple2 (One ("s", Bit)) (Tuple2 (One ("a", Bit)) (One ("b", Bit))))
-     (One ("o", Bit))
+   combinationalInterface "mux2_1"
+     (mkPort "s" Bit, (mkPort "a" Bit, mkPort "b" Bit))
+     (mkPort "o" Bit)
      [].
 
 Definition mux2_1_netlist :=
